proof/crypto_stream/chacha20/ref/ChaCha20_pavx2.ec
@@ -1,0 +1,1140 @@
+require import List Jasmin_model Int IntDiv CoreMap.
+require import Array16.
+require import WArray64.
+require import ChaCha20_pref ChaCha20_avx2_pv.
+
+module M = {
+  proc init_x2(key:W64.t, nonce:W64.t, counter:W32.t) : W32.t Array16.t * W32.t Array16.t = {
+    var st_1, st_2: W32.t Array16.t;
+    st_1 <@ ChaCha20_pref.M.init (key, nonce, counter);
+    st_2 <@ ChaCha20_pref.M.increment_counter(st_1);
+    return (st_1, st_2);
+  }
+
+  proc column_round_x2(k1_1 k1_2: W32.t Array16.t) : W32.t Array16.t * W32.t Array16.t = {
+    k1_1 <@  ChaCha20_pref.M.column_round(k1_1);
+    k1_2 <@  ChaCha20_pref.M.column_round(k1_2);
+    return (k1_1, k1_2);
+  }
+
+  proc diagonal_round_x2(k1_1 k1_2: W32.t Array16.t) : W32.t Array16.t * W32.t Array16.t = {
+    k1_1 <@  ChaCha20_pref.M.diagonal_round(k1_1);
+    k1_2 <@  ChaCha20_pref.M.diagonal_round(k1_2);
+    return (k1_1, k1_2);
+  }
+
+  proc rounds_x2_aux(k1_1 k1_2: W32.t Array16.t) : W32.t Array16.t * W32.t Array16.t = {
+    k1_1 <@ ChaCha20_pref.M.rounds(k1_1);
+    k1_2 <@ ChaCha20_pref.M.rounds(k1_2);
+    return (k1_1, k1_2);
+  }
+
+  proc rounds_x2(k1_1 k1_2: W32.t Array16.t) : W32.t Array16.t * W32.t Array16.t = {
+    var c : int;
+    c <- 0;
+    while (c < 10) {
+      (k1_1, k1_2) <- column_round_x2(k1_1, k1_2);
+      (k1_1, k1_2) <- diagonal_round_x2(k1_1, k1_2);
+      c <- c + 1;
+    }
+    return (k1_1, k1_2);
+  }
+
+  proc sum_states_x2(k1_1 k1_2 st_1 st_2: W32.t Array16.t) : W32.t Array16.t * W32.t Array16.t = {
+    var k1, k2 :  W32.t Array16.t;
+    k1 <@ ChaCha20_pref.M.sum_states(k1_1, st_1);
+    k2 <@ ChaCha20_pref.M.sum_states(k1_2, st_2);
+    return (k1, k2);
+  }
+    
+  proc copy_state_x4(st_1 st_2: W32.t Array16.t) : W32.t Array16.t * W32.t Array16.t = {
+    st_1.[12] <- st_1.[12] + W32.of_int 2;
+    st_2.[12] <- st_2.[12] + W32.of_int 2;
+    return (st_1, st_2);
+  }
+
+  proc rounds_x4 (st_1, st_2, st_3, st_4 :  W32.t Array16.t) = {
+    (st_1, st_2) <@ rounds_x2 (st_1, st_2);
+    (st_3, st_4) <@ rounds_x2 (st_3, st_4);
+    return (st_1, st_2, st_3, st_4);
+  }
+
+  proc sum_states_x4(k1_1 k1_2 k2_1 k2_2 st_1 st_2: W32.t Array16.t) = {
+    (k1_1, k1_2) = sum_states_x2(k1_1, k1_2, st_1, st_2);
+    (k2_1, k2_2) = sum_states_x2(k2_1, k2_2, st_1, st_2);
+    k2_1.[12] <- k2_1.[12] + W32.of_int 2;
+    k2_2.[12] <- k2_2.[12] + W32.of_int 2;
+    return (k1_1, k1_2, k2_1, k2_2);
+  }
+
+  proc chacha20_less_than_257(output:W64.t, plain:W64.t, len:W32.t,
+                               key:W64.t, nonce:W64.t, counter:W32.t) : unit = {
+    var st_1, st_2, st_3, st_4, k1_1, k1_2, k2_1, k2_2: W32.t Array16.t;
+    (st_1, st_2) <@ init_x2(key, nonce, counter);
+    if (W32.of_int 128 \ult len) {
+       (st_3, st_4) <@ copy_state_x4(st_1, st_2);
+       (k1_1, k1_2, k2_1, k2_2) <@ rounds_x4(st_1, st_2, st_3, st_4);
+       (k1_1, k1_2, k2_1, k2_2) <@ sum_states_x4(k1_1, k1_2, k2_1, k2_2, st_1, st_2);
+       (output, plain, len) <@ ChaCha20_avx2_pv.M.store_x2(output, plain, len, k1_1, k1_2);
+       ChaCha20_avx2_pv.M.store_x2_last(output, plain, len, k2_1, k2_2);
+    } else {
+      (k1_1, k1_2) <@ rounds_x2 (st_1, st_2);
+      (k1_1, k1_2) <@ sum_states_x2(k1_1, k1_2, st_1, st_2);
+      ChaCha20_avx2_pv.M.store_x2_last(output, plain, len, k1_1, k1_2);
+    } 
+  }
+
+  proc chacha20_more_than_256(output:W64.t, plain:W64.t, len:W32.t,
+                               key:W64.t, nonce:W64.t, counter:W32.t) : unit = {
+  }
+
+
+  proc chacha20_avx2(output:W64.t, plain:W64.t, len:W32.t,
+                               key:W64.t, nonce:W64.t, counter:W32.t) : unit = {
+    if (len \ult W32.of_int 257) {
+      chacha20_less_than_257(output, plain, len, key, nonce, counter);
+    } else {
+      chacha20_more_than_256(output, plain, len, key, nonce, counter);
+      
+    }
+  }
+}.
+
+equiv eq_chacha20_init_x2 : ChaCha20_pref.M.init ~ M.init_x2 : 
+   ={key, nonce, counter, Glob.mem} ==> res{1} = res{2}.`1 /\  res{2}.`2 = res{1}.[12 <- res{1}.[12] + W32.of_int 1].
+proof.
+  proc => /=.
+  inline ChaCha20_pref.M.increment_counter.
+  wp 10 1; conseq (_: st{1} = st_1{2}) => />.
+  by inline [tuple] *; sim.
+qed.
+
+equiv eq_chacha20_less_than_257 : ChaCha20_avx2_pv.M.chacha20_less_than_257 ~ M.chacha20_less_than_257 :
+   ={output, plain, len, key, nonce, counter, Glob.mem} ==> 
+   ={Glob.mem}.
+proof.
+  proc => /=.
+  seq 1 1 : (#pre /\ st_1{1} = st_1{2} /\ st_2{2} = st_1{1}.[12 <- st_1{1}.[12] + W32.of_int 1]).
+  + by call eq_chacha20_init_x2; skip.
+  if => //; last first.
+  + inline ChaCha20_avx2_pv.M.chacha20_less_than_128; sim.
+    swap{1} 7 -2. interleave{1} [6:1] [8:1] 2.  
+    inline [-tuple] M.sum_states_x2 ChaCha20_pref.M.increment_counter M.rounds_x2 ChaCha20_pref.M.rounds; sim.
+    swap{1} 11 3. swap{1} 11 -2.
+    wp; sp 9 2.  
+    transitivity * {1} {
+      c <- 0;
+      while (c < 10) {
+        k <@ ChaCha20_pref.M.round(k);
+        k0 <@ ChaCha20_pref.M.round(k0);
+        c <- c + 1;
+      }
+    }.
+    + smt(). + done.
+    + unroll for {1} 4;unroll for {1} 2;unroll for {2} 2.
+      by interleave{1} [1:2] [22:2] 10; sim.
+    while (#post /\ ={c}); last by auto.
+    inline [-tuple] ChaCha20_pref.M.round M.column_round_x2 M.diagonal_round_x2.
+    by swap{1} [5..6] -2; wp; sim />. 
+  
+ 
+
+inline ChaCha20_pref.M.rounds.
+ 
+    transitivity * {  
+inline [-tuple] ChaCha20_avx2_pv.M.chacha20_less_than_128 ChaCha20_avx2_pv.M.chacha20_body; sim.
+    inline{1} (2) ChaCha20_pref.M.increment_counter; wp.
+    swap{1} 8 -2. 
+    inline [-tuple] M.sum_states_x2; wp.
+    swap{1} [8..9] 1. swap{1} [9..11] 3. sim.
+    replace * {1} {_ as c1; (_ <@ _; _; _ <@ _) as c2} by 
+                  {c1; 
+                   (k,k0) <@ M.rounds_x2_aux(st0, st1);
+                   st2 <- st1; }.
+    + smt (). + done.
+    + by inline M.rounds_x2_aux; sim.
+    wp; call rounds_x2_aux_rounds_x2.
+    by inline ChaCha20_pref.M.increment_counter; auto.
+  inline{1} ChaCha20_avx2_pv.M.chacha20_between_128_255_1.
+  inline{1} [-tuple] ChaCha20_avx2_pv.M.chacha20_body ChaCha20_avx2_pv.M.chacha20_less_than_128.
+  swap{1} 11 -1. swap{1} [9..10] 10.
+  swap{1} 14 -2. swap{1} [8..12] -2.
+  swap{1} [19..24] 17.
+  swap{1} 23 -2. swap{1} [18..21] -1. swap{1} [16..20] -5.
+  swap{1} 31 -2. swap{1} [27..29] -1. swap{1} [25..28] -9.
+  swap{1} 21 1. swap{1} [22..25] 1. swap{1} [23..29] 1. 
+  inline{2} [-tuple] M.sum_states_x4 M.sum_states_x2; sim.
+  wp.
+  
+
+swap{1} [24..29] 1. swap{1} [25..
+  
+  swap{1} 16 -2.
+  
+
+qed.
+
+
+
+  inline [-tuple] M.rounds_x2 ChaCha20_pref.M.rounds.
+  
+    
+  inline 
+  
+  interleave{2} [2:1] [4:1] 2.
+  interleave{
+  transitivity{1}
+    {
+      output0 <- output;
+      plain0 <- plain;                             
+      len0 <- len;                               
+      st <- st_1;                                   
+      st0 <- st;                                     
+      st1 <@ ChaCha20_pref.M.increment_counter(st0);
+      k <@ ChaCha20_pref.M.rounds(st0); 
+      k <@ ChaCha20_avx2_pv.M.sum_states(k, st0);
+      k1_10 <- k;
+      st_20 <- st1;    
+      st2 <- st_20;                    
+      k0 <@ ChaCha20_pref.M.rounds(st2);
+      k0 <@ ChaCha20_avx2_pv.M.sum_states(k0, st2);
+    }
+    (={output, plain, len, st_1, Glob.mem} ==> ={k0, k1_10, len0, plain0, output0, Glob.mem})
+  
+    ((={output, plain, len, key, nonce, counter, Glob.mem} /\ ={st_1} /\ st_2{2} = st_1{1}.[12 <- st_1{1}.[12] + W32.one]) /\
+     ! ((of_int 128)%W32 \ult len{1}) ==>
+     k0{1} = k2{2} /\
+     k1_10{1} = k1{2} /\ len0{1} = len{2} /\ plain0{1} = plain{2} /\ output0{1} = output{2} /\ ={Glob.mem}) => //.
+   + smt().  
+   + by sim.
+   swap{1} [8 .. 9] 3; sim.
+   swap{1} [8..9] -1.
+   seq 8 0 : (#{/~k0{1}}{ ~ k{1}}post).
+   + by inline *;auto.
+   inline M.rounds_x2.
+   inline ChaCha20_pref.M.rounds.
+   inline M.column_round_x2 M.diagonal_round_x2.
+   sp; wp.
+   transitivity{2} {
+      while (c < 10) {                                
+         k1_12 <@ ChaCha20_pref.M.column_round(k1_11);  
+         k1_22 <@ ChaCha20_pref.M.column_round(k1_21);  
+         k1_11 <@ ChaCha20_pref.M.diagonal_round(k1_12);
+         k1_21 <@ ChaCha20_pref.M.diagonal_round(k1_22);
+         c <- c + 1;                                    
+       }                                               
+       (k1_1, k1_2) <- (k1_11, k1_21);
+     }
+   (k1_11{2} = st_1{2} /\
+  k1_21{2} = st_2{2} /\
+  c{2} = 0 /\
+  k1{1} = st0{1} /\
+  c{1} = W32.zero /\
+  st2{1} = st_2{2} /\
+  st0{1} = st_1{2} /\ len0{1} = len{2} /\ plain0{1} = plain{2} /\ output0{1} = output{2} /\ ={Glob.mem} ==>
+
+    k2{1} = k1_21{2} /\
+  st2{1} = st_2{2} /\
+  k{1} = k1_11{2} /\
+  st0{1} = st_1{2} /\ len0{1} = len{2} /\ plain0{1} = plain{2} /\ output0{1} = output{2} /\ ={Glob.mem})
+  (={c,k1_11, k1_12, Glob.mem, st_1, st_2, output, plain, len} ==> ={k1_11, k1_21, st_1, st_2, Glob.mem,output, plain, len}) => //. 
+  + smt().
+  + admit.
+  while (#pre).
+
+ 
+deadcode.
+constprop.
+
+
+ st0{1} = st_1{2} /\ st2{1} = st_2{2} /\ 
+
+len0{1} = len{2} /\ plain0{1} = plain{2} /\ output0{1} = output{2} /\ ={Glob.mem}
+   sim.
+  splittuple 
+
+
+
+
+
+  swap{1} 6 -3.
+equiv eq_chacha20_avx2 : ChaCha20_avx2_pv.M.chacha20_avx2 ~ M.chacha20_avx2 :
+   ={output, plain, len, key, nonce, counter, Glob.mem} ==> 
+   ={Glob.mem}.
+proof.
+  proc => /=.
+  if => //.
+
+  
+
+module M = {
+  proc shuffle_state_1 (st:W32.t Array16.t) : W32.t Array16.t = {
+    var st':W32.t Array16.t;
+    st'.[0]  <- st.[0];
+    st'.[1]  <- st.[1];
+    st'.[2]  <- st.[2];
+    st'.[3]  <- st.[3];
+             
+    st'.[4]  <- st.[5];
+    st'.[5]  <- st.[6];
+    st'.[6]  <- st.[7];
+    st'.[7]  <- st.[4];
+
+    st'.[8]  <- st.[10];
+    st'.[9]  <- st.[11];
+    st'.[10] <- st.[8];
+    st'.[11] <- st.[9];
+
+    st'.[12] <- st.[15];
+    st'.[13] <- st.[12];
+    st'.[14] <- st.[13];
+    st'.[15] <- st.[14];
+    return st';
+  }
+
+ proc reverse_shuffle_state_1 (st':W32.t Array16.t) : W32.t Array16.t = {
+    var st:W32.t Array16.t;
+    st.[0]  <- st'.[0];
+    st.[1]  <- st'.[1];
+    st.[2]  <- st'.[2];
+    st.[3]  <- st'.[3];
+                       
+    st.[5]  <- st'.[4];
+    st.[6]  <- st'.[5];
+    st.[7]  <- st'.[6];
+    st.[4]  <- st'.[7];
+                       
+    st.[10] <- st'.[8];
+    st.[11] <- st'.[9];
+    st.[8]  <- st'.[10];
+    st.[9]  <- st'.[11];
+                       
+    st.[15] <- st'.[12];
+    st.[12] <- st'.[13];
+    st.[13] <- st'.[14];
+    st.[14] <- st'.[15];
+    return st;
+  }
+
+ proc rotate_1(k:W32.t Array16.t, i r : int) :  W32.t Array16.t = {
+   k.[i + 0] <- W32.rol k.[i + 0] r;
+   k.[i + 1] <- W32.rol k.[i + 1] r;
+   k.[i + 2] <- W32.rol k.[i + 2] r;
+   k.[i + 3] <- W32.rol k.[i + 3] r;
+   return k;
+ }
+
+ proc line_1 (k:W32.t Array16.t, a b c r : int) : W32.t Array16.t = {
+   var i, a4, b4, c4 : int;
+   i <- 0;
+  
+   k.[a + 0] <-  k.[a + 0] + k.[b + 0];
+   k.[a + 1] <-  k.[a + 1] + k.[b + 1];
+   k.[a + 2] <-  k.[a + 2] + k.[b + 2];
+   k.[a + 3] <-  k.[a + 3] + k.[b + 3];
+
+   k.[c + 0] <-  k.[c + 0] `^` k.[a + 0];
+   k.[c + 1] <-  k.[c + 1] `^` k.[a + 1];
+   k.[c + 2] <-  k.[c + 2] `^` k.[a + 2];
+   k.[c + 3] <-  k.[c + 3] `^` k.[a + 3];
+
+   k <@ rotate_1(k, c, r);
+   return k;   
+ }
+
+ proc column_round_1 (k:W32.t Array16.t) : W32.t Array16.t = {
+   k <@ line_1(k, 0, 4, 12, 16);
+   k <@ line_1(k, 8, 12, 4, 12);
+   k <@ line_1(k, 0, 4, 12,  8);
+   k <@ line_1(k, 8, 12, 4,  7);
+  return k;
+ }
+
+ proc diagonal_round_1(k:W32.t Array16.t) : W32.t Array16.t = {
+   var k1, k2, k3 : W32.t Array16.t; 
+   k1 <@ shuffle_state_1(k);
+   k2 <@ column_round_1(k1);
+   k3 <@ reverse_shuffle_state_1(k2);
+   return k3;
+ }
+
+ proc round_1 (k:W32.t Array16.t) : W32.t Array16.t = {
+   var k1, k2 : W32.t Array16.t; 
+   k1 <@ column_round_1 (k);
+   k2 <@ diagonal_round_1 (k1);
+   return k2;
+ }
+
+ proc rounds_1 (k:W32.t Array16.t) : W32.t Array16.t = {
+   var c : int;
+   while (c < 20) {
+     k <@ round_1(k);
+     c <- c + 1;
+   }
+   return k;
+ }
+   
+ proc shuffle_state_2 (st1, st2:W32.t Array16.t) : W32.t Array16.t * W32.t Array16.t = {
+   st1 <@ shuffle_state_1(st1);
+   st2 <@ shuffle_state_1(st2);
+   return (st1, st2);
+ }
+
+ proc reverse_shuffle_state_2 (st1, st2:W32.t Array16.t) : W32.t Array16.t * W32.t Array16.t = {
+   st1 <@ reverse_shuffle_state_1(st1);
+   st2 <@ reverse_shuffle_state_1(st2);
+   return (st1, st2);
+ }
+
+
+ proc rotate_2 (k1 k2:W32.t Array16.t, i r : int) :  W32.t Array16.t * W32.t Array16.t = {
+   k1 <@ rotate_1(k1, i, r);
+   k2 <@ rotate_1(k2, i, r);
+   return (k1, k2);
+ }
+
+ proc line_2 (k1 k2:W32.t Array16.t, a b c r : int) :  W32.t Array16.t * W32.t Array16.t = {
+   k1 <@ line_1(k1, a, b, c, r);
+   k2 <@ line_1(k2, a, b, c, r);
+   return (k1, k2);
+ }
+
+ proc column_round_2 (k1 k2:W32.t Array16.t) : W32.t Array16.t  * W32.t Array16.t = {
+   (k1, k2) <@ line_2(k1, k2, 0, 4, 12, 16);
+   (k1, k2) <@ line_2(k1, k2, 8, 12, 4, 12);
+   (k1, k2) <@ line_2(k1, k2, 0, 4, 12,  8);
+   (k1, k2) <@ line_2(k1, k2, 8, 12, 4,  7);
+  return (k1, k2);
+ }
+
+ proc diagonal_round_2(k1, k2:W32.t Array16.t) : W32.t Array16.t * W32.t Array16.t = {
+   var k1_1, k1_2, k2_1, k2_2, k1_3, k2_3 : W32.t Array16.t; 
+   (k1_1, k2_2) <@ shuffle_state_2(k1, k2);
+   (k1_2, k2_2) <@ column_round_2(k1_1, k2_1);
+   (k1_3, k2_3) <@ reverse_shuffle_state_2(k2_1, k2_2);
+   return (k1_3, k2_3);
+ }
+
+ proc round_2 (k1 k2:W32.t Array16.t) : W32.t Array16.t * W32.t Array16.t = {
+   var k1_1, k1_2, k2_1, k2_2 : W32.t Array16.t; 
+   (k1_1, k2_1) <@ column_round_2 (k1, k2);
+   (k1_2, k2_2) <@ diagonal_round_2 (k1_1, k2_1);
+   return (k1_2, k2_2);
+ }
+
+ proc rounds_1_2 (k1 k2:W32.t Array16.t) : W32.t Array16.t * W32.t Array16.t = {
+   var c : int;
+   k1 <@ rounds_1(k1);
+   k2 <@ rounds_1(k2);
+   return (k1, k2);
+ }
+
+ proc rounds_2 (k1 k2:W32.t Array16.t) : W32.t Array16.t * W32.t Array16.t = {
+   var c : int;
+   while (c < 20) {
+     (k1, k2) <@ round_2(k1, k2);
+     c <- c + 1;
+   }
+   return (k1, k2);
+ }
+
+ proc chacha20_less_than_128 (output:W64.t, plain:W64.t, len:W32.t, st1 st2 : W32.t Array16.t) : unit = {
+   (k1,k2) <@ rounds_2 
+}.
+
+
+
+proc chacha20_less_than_128 (output:W64.t, plain:W64.t, len:W32.t, st : W32.t Array16.t) : unit = {
+     var k1_1:W32.t Array16.t;
+     var st_2:W32.t Array16.t;
+     var k1_2:W32.t Array16.t;
+     var st_3:W32.t Array16.t;
+     (k1_1, st_2) <@ chacha20_body (st);
+     (k1_2, st_3) <@ chacha20_body (st_2);
+     store_x2_last (output, plain, len, k1_1, k1_2);
+  }
+
+
+
+
+
+
+(* proc round_x2(k1:W32.t Array16.t, k2:W32.t Array16.t) : W32.t Array16.t *  W32.t Array16.t = {
+   (k1, k2) = column_round_x2  (k1, k2)
+   (k1, k2) = diagonal_round_x2(k1, k2)
+   return (k1, k2)
+ proc rounds_x2 *)
+}.
+
+(*
+hoare test k0 : M.id : k = k0 ==> Array16.all_eq k0 res.
+proof.
+  rewrite /Array16.all_eq /=.
+  proc. 
+  inline *; wp; skip => &hr heq /=.
+  rewrite heq //=.
+qed.
+*)
+
+equiv eq_column_round : ChaCha20_pref.M.column_round ~ M.column_round : ={k} ==> ={res}.
+proof.
+  conseq (_: Array16.all_eq res{1} res{2}).
+  + move=> &1 &2 ???; apply Array16.all_eq_eq.
+  rewrite /Array16.all_eq /=.
+  proc; inline *; wp; skip.
+  move=> &1 &2 heq; cbv delta; rewrite heq //=.
+qed.
+
+equiv diagonal_round_pref_shuffle1 : ChaCha20_pref.M.diagonal_round ~ M.diagonal_round :
+  ={k} ==> ={res}.
+proof.
+  conseq (_: Array16.all_eq res{1} res{2}).
+  + move=> &1 &2 ???; apply Array16.all_eq_eq.
+  rewrite /Array16.all_eq /=.
+  proc; inline *; wp; skip.
+  move => &1 &2 heq /=; rewrite heq //=.
+qed. 
+admitted.
+
+
+rewrite /Array16.all
+
+  
+
+abbrev bswap = W128.of_int 5233100606242806050955395731361295.
+
+
+module M = {
+  proc init (key:W64.t, nonce:W64.t, counter:W32.t) : W32.t Array16.t = {
+    var aux: int;
+    
+    var st:W32.t Array16.t;
+    var i:int;
+    st <- witness;
+    st.[0] <- (W32.of_int 1634760805);
+    st.[1] <- (W32.of_int 857760878);
+    st.[2] <- (W32.of_int 2036477234);
+    st.[3] <- (W32.of_int 1797285236);
+    i <- 0;
+    while (i < 8) {
+      st.[(4 + i)] <- (loadW32 Glob.mem (key + (W64.of_int (4 * i))));
+      i <- i + 1;
+    }
+    st.[12] <- counter;
+    i <- 0;
+    while (i < 3) {
+      st.[(13 + i)] <- (loadW32 Glob.mem (nonce + (W64.of_int (4 * i))));
+      i <- i + 1;
+    }
+    return (st);
+  }
+  
+  proc init_x2 (key:W64.t, nonce:W64.t, counter:W32.t) : W32.t Array16.t *
+                                                         W32.t Array16.t = {
+    
+    var st_1:W32.t Array16.t;
+    var st_2:W32.t Array16.t;
+    st_1 <- witness;
+    st_2 <- witness;
+    st_1 <@ init (key, nonce, counter);
+    counter <- (counter + (W32.of_int 1));
+    st_2 <@ init (key, nonce, counter);
+    return (st_1, st_2);
+  }
+  
+  proc init_x8 (key:W64.t, nonce:W64.t, counter:W32.t) : W32.t Array16.t *
+                                                         W32.t Array16.t *
+                                                         W32.t Array16.t *
+                                                         W32.t Array16.t *
+                                                         W32.t Array16.t *
+                                                         W32.t Array16.t *
+                                                         W32.t Array16.t *
+                                                         W32.t Array16.t = {
+    
+    var st_1:W32.t Array16.t;
+    var st_2:W32.t Array16.t;
+    var st_3:W32.t Array16.t;
+    var st_4:W32.t Array16.t;
+    var st_5:W32.t Array16.t;
+    var st_6:W32.t Array16.t;
+    var st_7:W32.t Array16.t;
+    var st_8:W32.t Array16.t;
+    st_1 <- witness;
+    st_2 <- witness;
+    st_3 <- witness;
+    st_4 <- witness;
+    st_5 <- witness;
+    st_6 <- witness;
+    st_7 <- witness;
+    st_8 <- witness;
+    st_1 <@ init (key, nonce, counter);
+    counter <- (counter + (W32.of_int 1));
+    st_2 <@ init (key, nonce, counter);
+    counter <- (counter + (W32.of_int 1));
+    st_3 <@ init (key, nonce, counter);
+    counter <- (counter + (W32.of_int 1));
+    st_4 <@ init (key, nonce, counter);
+    counter <- (counter + (W32.of_int 1));
+    st_5 <@ init (key, nonce, counter);
+    counter <- (counter + (W32.of_int 1));
+    st_6 <@ init (key, nonce, counter);
+    counter <- (counter + (W32.of_int 1));
+    st_7 <@ init (key, nonce, counter);
+    counter <- (counter + (W32.of_int 1));
+    st_8 <@ init (key, nonce, counter);
+    return (st_1, st_2, st_3, st_4, st_5, st_6, st_7, st_8);
+  }
+  
+  proc copy_state (st:W32.t Array16.t) : W32.t Array16.t = {
+    
+    var k:W32.t Array16.t;
+    k <- witness;
+    k <- st;
+    return (k);
+  }
+  
+  proc copy_state_x2 (st_1:W32.t Array16.t, st_2:W32.t Array16.t) : W32.t Array16.t *
+                                                                    W32.t Array16.t = {
+    
+    var k_1:W32.t Array16.t;
+    var k_2:W32.t Array16.t;
+    k_1 <- witness;
+    k_2 <- witness;
+    k_1 <@ copy_state (st_1);
+    k_2 <@ copy_state (st_2);
+    return (k_1, k_2);
+  }
+  
+  proc copy_state_x4 (st_1:W32.t Array16.t, st_2:W32.t Array16.t) : W32.t Array16.t *
+                                                                    W32.t Array16.t *
+                                                                    W32.t Array16.t *
+                                                                    W32.t Array16.t = {
+    
+    var k_1:W32.t Array16.t;
+    var k_2:W32.t Array16.t;
+    var k_3:W32.t Array16.t;
+    var k_4:W32.t Array16.t;
+    k_1 <- witness;
+    k_2 <- witness;
+    k_3 <- witness;
+    k_4 <- witness;
+    k_1 <@ copy_state (st_1);
+    k_2 <@ copy_state (st_2);
+    k_3 <@ copy_state (st_1);
+    k_4 <@ copy_state (st_2);
+    k_3.[12] <- (k_3.[12] + (W32.of_int 2));
+    k_4.[12] <- (k_4.[12] + (W32.of_int 2));
+    return (k_1, k_2, k_3, k_4);
+  }
+  
+  proc copy_state_x8 (st_1:W32.t Array16.t, st_2:W32.t Array16.t,
+                      st_3:W32.t Array16.t, st_4:W32.t Array16.t,
+                      st_5:W32.t Array16.t, st_6:W32.t Array16.t,
+                      st_7:W32.t Array16.t, st_8:W32.t Array16.t) : W32.t Array16.t *
+                                                                    W32.t Array16.t *
+                                                                    W32.t Array16.t *
+                                                                    W32.t Array16.t *
+                                                                    W32.t Array16.t *
+                                                                    W32.t Array16.t *
+                                                                    W32.t Array16.t *
+                                                                    W32.t Array16.t = {
+    
+    var k_1:W32.t Array16.t;
+    var k_2:W32.t Array16.t;
+    var k_3:W32.t Array16.t;
+    var k_4:W32.t Array16.t;
+    var k_5:W32.t Array16.t;
+    var k_6:W32.t Array16.t;
+    var k_7:W32.t Array16.t;
+    var k_8:W32.t Array16.t;
+    k_1 <- witness;
+    k_2 <- witness;
+    k_3 <- witness;
+    k_4 <- witness;
+    k_5 <- witness;
+    k_6 <- witness;
+    k_7 <- witness;
+    k_8 <- witness;
+    k_1 <@ copy_state (st_1);
+    k_2 <@ copy_state (st_2);
+    k_3 <@ copy_state (st_3);
+    k_4 <@ copy_state (st_4);
+    k_5 <@ copy_state (st_5);
+    k_6 <@ copy_state (st_6);
+    k_7 <@ copy_state (st_7);
+    k_8 <@ copy_state (st_8);
+    return (k_1, k_2, k_3, k_4, k_5, k_6, k_7, k_8);
+  }
+  
+  proc sum_states (k:W32.t Array16.t, st:W32.t Array16.t) : W32.t Array16.t = {
+    var aux: int;
+    
+    var i:int;
+    
+    i <- 0;
+    while (i < 16) {
+      k.[i] <- (k.[i] + st.[i]);
+      i <- i + 1;
+    }
+    return (k);
+  }
+  
+  proc sum_states_x2 (k_1:W32.t Array16.t, k_2:W32.t Array16.t,
+                      st_1:W32.t Array16.t, st_2:W32.t Array16.t) : W32.t Array16.t *
+                                                                    W32.t Array16.t = {
+    
+    
+    
+    k_1 <@ sum_states (k_1, st_1);
+    k_2 <@ sum_states (k_2, st_2);
+    return (k_1, k_2);
+  }
+  
+  proc sum_states_x4 (k1_1:W32.t Array16.t, k1_2:W32.t Array16.t,
+                      k2_1:W32.t Array16.t, k2_2:W32.t Array16.t,
+                      st_1:W32.t Array16.t, st_2:W32.t Array16.t) : W32.t Array16.t *
+                                                                    W32.t Array16.t *
+                                                                    W32.t Array16.t *
+                                                                    W32.t Array16.t = {
+    
+    
+    
+    (k1_1, k1_2) <@ sum_states_x2 (k1_1, k1_2, st_1, st_2);
+    (k2_1, k2_2) <@ sum_states_x2 (k2_1, k2_2, st_1, st_2);
+    k2_1.[12] <- (k2_1.[12] + (W32.of_int 2));
+    k2_2.[12] <- (k2_2.[12] + (W32.of_int 2));
+    return (k1_1, k1_2, k2_1, k2_2);
+  }
+  
+  proc sum_states_x8 (k_1:W32.t Array16.t, k_2:W32.t Array16.t,
+                      k_3:W32.t Array16.t, k_4:W32.t Array16.t,
+                      k_5:W32.t Array16.t, k_6:W32.t Array16.t,
+                      k_7:W32.t Array16.t, k_8:W32.t Array16.t,
+                      st_1:W32.t Array16.t, st_2:W32.t Array16.t,
+                      st_3:W32.t Array16.t, st_4:W32.t Array16.t,
+                      st_5:W32.t Array16.t, st_6:W32.t Array16.t,
+                      st_7:W32.t Array16.t, st_8:W32.t Array16.t) : W32.t Array16.t *
+                                                                    W32.t Array16.t *
+                                                                    W32.t Array16.t *
+                                                                    W32.t Array16.t *
+                                                                    W32.t Array16.t *
+                                                                    W32.t Array16.t *
+                                                                    W32.t Array16.t *
+                                                                    W32.t Array16.t = {
+    
+    
+    
+    k_1 <@ sum_states (k_1, st_1);
+    k_2 <@ sum_states (k_2, st_2);
+    k_3 <@ sum_states (k_3, st_3);
+    k_4 <@ sum_states (k_4, st_4);
+    k_5 <@ sum_states (k_5, st_5);
+    k_6 <@ sum_states (k_6, st_6);
+    k_7 <@ sum_states (k_7, st_7);
+    k_8 <@ sum_states (k_8, st_8);
+    return (k_1, k_2, k_3, k_4, k_5, k_6, k_7, k_8);
+  }
+  
+  proc update_ptr (output:W64.t, plain:W64.t, len:W32.t, n:int) : W64.t *
+                                                                  W64.t *
+                                                                  W32.t = {
+    
+    
+    
+    output <- (output + (W64.of_int n));
+    plain <- (plain + (W64.of_int n));
+    len <- (len - (W32.of_int n));
+    return (output, plain, len);
+  }
+  
+  proc store (output:W64.t, plain:W64.t, len:W32.t, k:W32.t Array16.t) : 
+  W64.t * W64.t * W32.t = {
+    var aux: int;
+    
+    var i:int;
+    
+    i <- 0;
+    while (i < 16) {
+      k.[i] <- (k.[i] `^` (loadW32 Glob.mem (plain + (W64.of_int (4 * i)))));
+      Glob.mem <- storeW32 Glob.mem (output + (W64.of_int (4 * i))) k.[i];
+      i <- i + 1;
+    }
+    (output, plain, len) <@ update_ptr (output, plain, len, 64);
+    return (output, plain, len);
+  }
+  
+  proc store_last (output:W64.t, plain:W64.t, len:W32.t, k:W32.t Array16.t) : unit = {
+    
+    var s_k:W32.t Array16.t;
+    var j:W64.t;
+    var pi:W8.t;
+    s_k <- witness;
+    s_k <- k;
+    j <- (W64.of_int 0);
+    
+    while (((truncateu32 j) \ult len)) {
+      pi <- (loadW8 Glob.mem (plain + j));
+      pi <-
+      (pi `^` (get8 (WArray64.init32 (fun i => s_k.[i])) (W64.to_uint j)));
+      Glob.mem <- storeW8 Glob.mem (output + j) pi;
+      j <- (j + (W64.of_int 1));
+    }
+    return ();
+  }
+  
+  proc store_x2 (output:W64.t, plain:W64.t, len:W32.t, k_1:W32.t Array16.t,
+                 k_2:W32.t Array16.t) : W64.t * W64.t * W32.t = {
+    
+    
+    
+    (output, plain, len) <@ store (output, plain, len, k_1);
+    (output, plain, len) <@ store (output, plain, len, k_2);
+    return (output, plain, len);
+  }
+  
+  proc store_x2_last (output:W64.t, plain:W64.t, len:W32.t,
+                      k_1:W32.t Array16.t, k_2:W32.t Array16.t) : unit = {
+    
+    var r:W32.t Array16.t;
+    r <- witness;
+    r <- k_1;
+    if (((W32.of_int 64) \ule len)) {
+      (output, plain, len) <@ store (output, plain, len, r);
+      r <- k_2;
+    } else {
+      
+    }
+    store_last (output, plain, len, r);
+    return ();
+  }
+  
+  proc store_x4 (output:W64.t, plain:W64.t, len:W32.t, k_1:W32.t Array16.t,
+                 k_2:W32.t Array16.t, k_3:W32.t Array16.t,
+                 k_4:W32.t Array16.t) : W64.t * W64.t * W32.t = {
+    
+    
+    
+    (output, plain, len) <@ store (output, plain, len, k_1);
+    (output, plain, len) <@ store (output, plain, len, k_2);
+    (output, plain, len) <@ store (output, plain, len, k_3);
+    (output, plain, len) <@ store (output, plain, len, k_4);
+    return (output, plain, len);
+  }
+  
+  proc store_x4_last (output:W64.t, plain:W64.t, len:W32.t,
+                      k_1:W32.t Array16.t, k_2:W32.t Array16.t,
+                      k_3:W32.t Array16.t, k_4:W32.t Array16.t) : unit = {
+    
+    var r_1:W32.t Array16.t;
+    var r_2:W32.t Array16.t;
+    r_1 <- witness;
+    r_2 <- witness;
+    r_1 <- k_1;
+    r_2 <- k_2;
+    if (((W32.of_int 128) \ule len)) {
+      (output, plain, len) <@ store_x2 (output, plain, len, r_1, r_2);
+      r_1 <- k_3;
+      r_2 <- k_4;
+    } else {
+      
+    }
+    store_x2_last (output, plain, len, r_1, r_2);
+    return ();
+  }
+  
+  proc store_x8 (output:W64.t, plain:W64.t, len:W32.t, k_1:W32.t Array16.t,
+                 k_2:W32.t Array16.t, k_3:W32.t Array16.t,
+                 k_4:W32.t Array16.t, k_5:W32.t Array16.t,
+                 k_6:W32.t Array16.t, k_7:W32.t Array16.t,
+                 k_8:W32.t Array16.t) : W64.t * W64.t * W32.t = {
+    
+    
+    
+    (output, plain, len) <@ store (output, plain, len, k_1);
+    (output, plain, len) <@ store (output, plain, len, k_2);
+    (output, plain, len) <@ store (output, plain, len, k_3);
+    (output, plain, len) <@ store (output, plain, len, k_4);
+    (output, plain, len) <@ store (output, plain, len, k_5);
+    (output, plain, len) <@ store (output, plain, len, k_6);
+    (output, plain, len) <@ store (output, plain, len, k_7);
+    (output, plain, len) <@ store (output, plain, len, k_8);
+    return (output, plain, len);
+  }
+  
+  proc store_x8_last (output:W64.t, plain:W64.t, len:W32.t,
+                      k_1:W32.t Array16.t, k_2:W32.t Array16.t,
+                      k_3:W32.t Array16.t, k_4:W32.t Array16.t,
+                      k_5:W32.t Array16.t, k_6:W32.t Array16.t,
+                      k_7:W32.t Array16.t, k_8:W32.t Array16.t) : unit = {
+    
+    var r_1:W32.t Array16.t;
+    var r_2:W32.t Array16.t;
+    var r_3:W32.t Array16.t;
+    var r_4:W32.t Array16.t;
+    r_1 <- witness;
+    r_2 <- witness;
+    r_3 <- witness;
+    r_4 <- witness;
+    r_1 <- k_1;
+    r_2 <- k_2;
+    r_3 <- k_3;
+    r_4 <- k_4;
+    if (((W32.of_int 256) \ule len)) {
+      (output, plain, len) <@ store_x4 (output, plain, len, r_1, r_2, r_3,
+      r_4);
+      r_1 <- k_5;
+      r_2 <- k_6;
+      r_3 <- k_7;
+      r_4 <- k_8;
+    } else {
+      
+    }
+    store_x4_last (output, plain, len, r_1, r_2, r_3, r_4);
+    return ();
+  }
+  
+  proc increment_counter (st:W32.t Array16.t) : W32.t Array16.t = {
+    
+    
+    
+    st.[12] <- (st.[12] + (W32.of_int 8));
+    return (st);
+  }
+  
+  proc increment_counter_x8 (st_1:W32.t Array16.t, st_2:W32.t Array16.t,
+                             st_3:W32.t Array16.t, st_4:W32.t Array16.t,
+                             st_5:W32.t Array16.t, st_6:W32.t Array16.t,
+                             st_7:W32.t Array16.t, st_8:W32.t Array16.t) : 
+  W32.t Array16.t * W32.t Array16.t * W32.t Array16.t * W32.t Array16.t *
+  W32.t Array16.t * W32.t Array16.t * W32.t Array16.t * W32.t Array16.t = {
+    
+    
+    
+    st_1 <@ increment_counter (st_1);
+    st_2 <@ increment_counter (st_2);
+    st_3 <@ increment_counter (st_3);
+    st_4 <@ increment_counter (st_4);
+    st_5 <@ increment_counter (st_5);
+    st_6 <@ increment_counter (st_6);
+    st_7 <@ increment_counter (st_7);
+    st_8 <@ increment_counter (st_8);
+    return (st_1, st_2, st_3, st_4, st_5, st_6, st_7, st_8);
+  }
+  
+  proc line (k:W32.t Array16.t, a:int, b:int, c:int, r:int) : W32.t Array16.t = {
+    var aux_0: bool;
+    var aux: bool;
+    var aux_1: W32.t;
+    
+    var  _0:bool;
+    var  _1:bool;
+    
+    k.[a] <- (k.[a] + k.[b]);
+    k.[c] <- (k.[c] `^` k.[a]);
+    (aux_0, aux, aux_1) <- x86_ROL_32 k.[c] (W8.of_int r);
+     _0 <- aux_0;
+     _1 <- aux;
+    k.[c] <- aux_1;
+    return (k);
+  }
+  
+  proc quarter_round (k:W32.t Array16.t, a:int, b:int, c:int, d:int) : W32.t Array16.t = {  
+    k <@ line (k, a, b, d, 16);
+    k <@ line (k, c, d, b, 12);
+    k <@ line (k, a, b, d, 8);
+    k <@ line (k, c, d, b, 7);
+    return (k);
+  }
+  
+  proc rounds (k:W32.t Array16.t) : W32.t Array16.t = {
+    
+    var c:W32.t;
+    
+    c <- (W32.of_int 0);
+    
+    while ((c \ult (W32.of_int 10))) {
+      k <@ quarter_round (k, 0, 4, 8, 12);
+      k <@ quarter_round (k, 2, 6, 10, 14);
+      k <@ quarter_round (k, 1, 5, 9, 13);
+      k <@ quarter_round (k, 3, 7, 11, 15);
+      k <@ quarter_round (k, 1, 6, 11, 12);
+      k <@ quarter_round (k, 0, 5, 10, 15);
+      k <@ quarter_round (k, 2, 7, 8, 13);
+      k <@ quarter_round (k, 3, 4, 9, 14);
+      c <- (c + (W32.of_int 1));
+    }
+    return (k);
+  }
+  
+  proc round_x2_body (k_1:W32.t Array16.t, k_2:W32.t Array16.t) : W32.t Array16.t *
+                                                              W32.t Array16.t = {
+    (k_1, k_2) = column_round_x2(k, r16, r8);
+    (k_1, k_2) = diagonal_round_x2(k, r16, r8);
+    return (k_1, k_2);
+  }
+
+  proc rounds_x2_body (k_1:W32.t Array16.t, k_2:W32.t Array16.t) : W32.t Array16.t *
+                                                              W32.t Array16.t = {
+    var c : int;
+    c = 0;
+    while (c < 10) {
+      (k_1, k_2) <- round_x2(k_1, k_2);
+      c <- c + 1;
+    }
+    return (k_1, k_2);
+  }
+  
+  proc rounds_x4 (k_1:W32.t Array16.t, k_2:W32.t Array16.t,
+                  k_3:W32.t Array16.t, k_4:W32.t Array16.t) : W32.t Array16.t *
+                                                              W32.t Array16.t *
+                                                              W32.t Array16.t *
+                                                              W32.t Array16.t = {
+    
+    
+    
+    k_1 <@ rounds (k_1);
+    k_2 <@ rounds (k_2);
+    k_3 <@ rounds (k_3);
+    k_4 <@ rounds (k_4);
+    return (k_1, k_2, k_3, k_4);
+  }
+  
+  proc rounds_x8 (k_1:W32.t Array16.t, k_2:W32.t Array16.t,
+                  k_3:W32.t Array16.t, k_4:W32.t Array16.t,
+                  k_5:W32.t Array16.t, k_6:W32.t Array16.t,
+                  k_7:W32.t Array16.t, k_8:W32.t Array16.t) : W32.t Array16.t *
+                                                              W32.t Array16.t *
+                                                              W32.t Array16.t *
+                                                              W32.t Array16.t *
+                                                              W32.t Array16.t *
+                                                              W32.t Array16.t *
+                                                              W32.t Array16.t *
+                                                              W32.t Array16.t = {
+    
+    
+    
+    k_1 <@ rounds (k_1);
+    k_2 <@ rounds (k_2);
+    k_3 <@ rounds (k_3);
+    k_4 <@ rounds (k_4);
+    k_5 <@ rounds (k_5);
+    k_6 <@ rounds (k_6);
+    k_7 <@ rounds (k_7);
+    k_8 <@ rounds (k_8);
+    return (k_1, k_2, k_3, k_4, k_5, k_6, k_7, k_8);
+  }
+  
+  proc chacha20_more_than_256 (output:W64.t, plain:W64.t, len:W32.t,
+                               key:W64.t, nonce:W64.t, counter:W32.t) : unit = {
+    
+    var st_1:W32.t Array16.t;
+    var st_2:W32.t Array16.t;
+    var st_3:W32.t Array16.t;
+    var st_4:W32.t Array16.t;
+    var st_5:W32.t Array16.t;
+    var st_6:W32.t Array16.t;
+    var st_7:W32.t Array16.t;
+    var st_8:W32.t Array16.t;
+    var k_1:W32.t Array16.t;
+    var k_2:W32.t Array16.t;
+    var k_3:W32.t Array16.t;
+    var k_4:W32.t Array16.t;
+    var k_5:W32.t Array16.t;
+    var k_6:W32.t Array16.t;
+    var k_7:W32.t Array16.t;
+    var k_8:W32.t Array16.t;
+    k_1 <- witness;
+    k_2 <- witness;
+    k_3 <- witness;
+    k_4 <- witness;
+    k_5 <- witness;
+    k_6 <- witness;
+    k_7 <- witness;
+    k_8 <- witness;
+    st_1 <- witness;
+    st_2 <- witness;
+    st_3 <- witness;
+    st_4 <- witness;
+    st_5 <- witness;
+    st_6 <- witness;
+    st_7 <- witness;
+    st_8 <- witness;
+    (st_1, st_2, st_3, st_4, st_5, st_6, st_7, st_8) <@ init_x8 (key, nonce,
+    counter);
+    
+    while (((W32.of_int 512) \ule len)) {
+      (k_1, k_2, k_3, k_4, k_5, k_6, k_7, k_8) <@ copy_state_x8 (st_1, st_2,
+      st_3, st_4, st_5, st_6, st_7, st_8);
+      (k_1, k_2, k_3, k_4, k_5, k_6, k_7, k_8) <@ rounds_x8 (k_1, k_2, k_3,
+      k_4, k_5, k_6, k_7, k_8);
+      (k_1, k_2, k_3, k_4, k_5, k_6, k_7, k_8) <@ sum_states_x8 (k_1, k_2,
+      k_3, k_4, k_5, k_6, k_7, k_8, st_1, st_2, st_3, st_4, st_5, st_6, st_7,
+      st_8);
+      (output, plain, len) <@ store_x8 (output, plain, len, k_1, k_2, k_3,
+      k_4, k_5, k_6, k_7, k_8);
+      (st_1, st_2, st_3, st_4, st_5, st_6, st_7,
+      st_8) <@ increment_counter_x8 (st_1, st_2, st_3, st_4, st_5, st_6,
+      st_7, st_8);
+    }
+    if (((W32.of_int 0) \ult len)) {
+      (k_1, k_2, k_3, k_4, k_5, k_6, k_7, k_8) <@ copy_state_x8 (st_1, st_2,
+      st_3, st_4, st_5, st_6, st_7, st_8);
+      (k_1, k_2, k_3, k_4, k_5, k_6, k_7, k_8) <@ rounds_x8 (k_1, k_2, k_3,
+      k_4, k_5, k_6, k_7, k_8);
+      (k_1, k_2, k_3, k_4, k_5, k_6, k_7, k_8) <@ sum_states_x8 (k_1, k_2,
+      k_3, k_4, k_5, k_6, k_7, k_8, st_1, st_2, st_3, st_4, st_5, st_6, st_7,
+      st_8);
+      store_x8_last (output, plain, len, k_1, k_2, k_3, k_4, k_5, k_6, k_7,
+      k_8);
+    } else {
+      
+    }
+    return ();
+  }
+  
+  proc chacha20_less_than_257 (output:W64.t, plain:W64.t, len:W32.t,
+                               key:W64.t, nonce:W64.t, counter:W32.t) : unit = {
+    
+    var st_1:W32.t Array16.t;
+    var st_2:W32.t Array16.t;
+    var k1_1:W32.t Array16.t;
+    var k1_2:W32.t Array16.t;
+    var k2_1:W32.t Array16.t;
+    var k2_2:W32.t Array16.t;
+    k1_1 <- witness;
+    k1_2 <- witness;
+    k2_1 <- witness;
+    k2_2 <- witness;
+    st_1 <- witness;
+    st_2 <- witness;
+    (st_1, st_2) <@ init_x2 (key, nonce, counter);
+    if (((W32.of_int 128) \ult len)) {
+      (k1_1, k1_2, k2_1, k2_2) <@ copy_state_x4 (st_1, st_2);
+      (k1_1, k1_2, k2_1, k2_2) <@ rounds_x4 (k1_1, k1_2, k2_1, k2_2);
+      (k1_1, k1_2, k2_1, k2_2) <@ sum_states_x4 (k1_1, k1_2, k2_1, k2_2,
+      st_1, st_2);
+      (output, plain, len) <@ store_x2 (output, plain, len, k1_1, k1_2);
+      store_x2_last (output, plain, len, k2_1, k2_2);
+    } else {
+      (k1_1, k1_2) <@ copy_state_x2 (st_1, st_2);
+      (k1_1, k1_2) <@ rounds_x2 (k1_1, k1_2);
+      (k1_1, k1_2) <@ sum_states_x2 (k1_1, k1_2, st_1, st_2);
+      store_x2_last (output, plain, len, k1_1, k1_2);
+    }
+    return ();
+  }
+  
+  proc chacha20_avx2 (output:W64.t, plain:W64.t, len:W32.t, key:W64.t,
+                      nonce:W64.t, counter:W32.t) : unit = {
+    
+    
+    
+    if ((len \ult (W32.of_int 257))) {
+      chacha20_less_than_257 (output, plain, len, key, nonce, counter);
+    } else {
+      chacha20_more_than_256 (output, plain, len, key, nonce, counter);
+    }
+    return ();
+  }
+}.
+
